change endian lemma

code/ecdsap256sha2/Hacl.Spec.ECDSA.fst
@@ -378,6 +378,34 @@ let changeEndian i =
           Lib.Sequence.upd o 3 zero
 
 
+val changeEndianLemma: k: lseq uint64 4 -> Lemma 
+  (nat_from_intseq_le (changeEndian k) == nat_from_intseq_be k)
+
+let changeEndianLemma k = 
+  let k0 = changeEndian k in 
+  
+  nat_from_intseq_be_slice_lemma (slice k 2 4) 1;
+  nat_from_intseq_be_slice_lemma (slice k 1 4) 1;
+  nat_from_intseq_be_slice_lemma k 1;
+  
+  nat_from_intseq_be_lemma0 (slice k 0 1);
+  nat_from_intseq_be_lemma0 (slice k 1 2);
+  nat_from_intseq_be_lemma0 (slice k 2 3);
+  nat_from_intseq_be_lemma0 (slice k 3 4);
+  
+  nat_from_intseq_le_slice_lemma (slice k0 2 4) 1;
+  nat_from_intseq_le_slice_lemma (slice k0 1 4) 1;
+  nat_from_intseq_le_slice_lemma k0 1;
+  
+  nat_from_intseq_le_lemma0 (slice k0 0 1);
+  nat_from_intseq_le_lemma0 (slice k0 1 2);
+  nat_from_intseq_le_lemma0 (slice k0 2 3);
+  nat_from_intseq_le_lemma0 (slice k0 3 4);
+
+  assert_norm (pow2 (2 * 64) * pow2 64 == pow2 (3 * 64))
+
+
+
 val verifyQValidCurvePointSpec:
   publicKey:tuple3 nat nat nat{~(isPointAtInfinity publicKey)} -> bool
 
